<?xml version="1.0" encoding="UTF-8"?>
<rdf:RDF xmlns:rdf="http://www.w3.org/1999/02/22-rdf-syntax-ns#" xmlns:skos="http://www.w3.org/2004/02/skos/core#" xmlns:owl="http://www.w3.org/2002/07/owl#" xmlns:xsd="http://www.w3.org/2001/XMLSchema#" xmlns:swrl="http://www.w3.org/2003/11/swrl#" xmlns:swrlb="http://www.w3.org/2003/11/swrlb#" xmlns:rdfs="http://www.w3.org/2000/01/rdf-schema#" xml:base="https://takin.solutions/ontologies/CRMcpr/">
<owl:versionInfo>RDFs Implementation (November 2023) of CRMcpr 1.5.1</owl:versionInfo>
<rdfs:comment xml:lang="en">
Scope  Creative Processes Representation Conceptual Reference Model (CRMcpr) is an ontological model harmonizing to the CIDOC CRM family of models that aims to facilitate the representation and integration of information related to creative processes and the materialization of ideas into reality. It has a particular focus on creative processes.  The presently proposed model and its related classes and properties have been modelled to cover architectural practice, artistic production, and design activities considered broadly.  Examples Used  In order to illustrate the ontology's use, the specification provides a related set of examples from architecture, the rebuild project on the site of the World Trade Centre, NY, and art the "Gates of Hell" by Rodin. Future editions aim to carry examples from additional fields.  Compatibility and Nomenclature  This unofficial extension of the CIDOC CRM is formulated in relation to:    CIDOC CRM v.7.1.2  FRBRoo v.2.4    The specification consists of a set of declarations for formalized classes and properties that extend the CIDOC CRM and the above official extensions.   Please note that FRBRoo 2.4 was formulated originally in relation to CIDOC CRM 6.2. In order to harmonize to the latest CIDOC CRM while using the FRBRoo modelling strategy we have ensured to use only classes and properties that are compatible across these two models. We choose to retain the modelling patterns of FRBRoo rather than the new model LRMoo which further restricts its scope to only library practice and loses many of the features that interest us in the modelling of creative process.  Adopting the conventions of the CIDOC CRM each class and property have been given an identifier in addition to their names. The naming convention adopted for this extension is:  CC = class  CP = property  The choice of these names was arbitrary, making a conceptual connection with the official CRM representation while clearly distinguishing the new classes and properties from those of either CRM base or its official extensions.  Namespace  https://takin.solutions/ontologies/crmcpr   Maintenance and Archiving  CRMcpr is an actively maintained ontology. It is our aim to develop publicaly and participatively, learning from and engaging with the scholarly community that adopts it. Towards this end we maintain the ontology with the following processes and relative tools.  Ontology Development  We adopt the OntoMe tool developed by LARHRA to manage the ontology and produce editions. This ensures a consistent management of the ontology and provides a public space to engage in revisions.  The maintenace space for the ontology can be found here: https://ontome.net/project/30   Issue Management and Revision Storage  We adopt github as a platform for inviting and managing issues related to the ontology as well as providing an active place to be able to access the latest edition of the ontology, its specification and relevant documentation.  The address for the github repository is: https://github.com/takinsolutions/crmcpr   Acknowledgements  The initiative for creating, developing and maintaining this ontology is made possible by important on-going funding and institutional commitment, which is gratefully acknowledged here.  Funding Support    The development/creation of the initial version (v1.0) of CRMcpr has been jointly funded by Swiss Art Research Infrastructure (SARI) and the University of Zurich’s Digital Society Initiative (DSI)  The continued development and enrichment of the latest version (v1.5) has been funded as part of the Open Research Data (ORD) initiative by swissuniversities.    Institutional Support:  The continuous maintenance and promotion of CRMcpr is made possible by the initial and on-going commitment of its institutional partners to this task.    Takin.solutions  Swiss Art Research Infrastructure - University of Zurich  UMR 3495 CNRS/MC MAP     
This ontology is supported and matained by the Swiss Art Research Institute and Takin.solutions.    
    
Exported from and adapted from OntoME: CRM for Creative Processes Representation Version 1.5.1
Official Namespace : https://takin.solutions/ontologies/CRMcpr/
</rdfs:comment>
  <rdfs:Class rdf:about="https://takin.solutions/ontologies/CRMcpr/CC1_Model">
    <skos:notation rdf:datatype="http://www.w3.org/2001/XMLSchema#string">CC1</skos:notation>
    <rdfs:comment xml:lang="en" rdf:datatype="http://www.w3.org/2001/XMLSchema#string">This class comprises the particularly expressed, immaterial, intellectual content of objects created during the creative design phase in order to represent aesthetic concepts. The propositional content contained in a model provides information regarding an overall CC13 Design Concept and can be used to understand some aspect of the creator’s intent. Instances of this class are information objects produced as  a result of design processes (instances of F28 Expression Creation) undertaken in relation to the goals of an instance of an overall CC15 Design Conception activity which, in turn, typically intends to comply with the specifications of an instance of CC6 Programme. As a subclass of F22 Self-Contained Expression, an instance of CC1 Model realizes, in whole or in part, the propositional content of the instance of CC13 Design Concept. As a subclass of CC5 Formulation, an instance of CC1 Model may function to project representations of the relations of space and materiality of the CC13 Design Concept, via CC12 Event Trigger Template, such that these representations can be used as guides for their eventual realization in some manufactured object.
 </rdfs:comment>
    <rdfs:label xml:lang="en">Model</rdfs:label>
    <rdfs:subClassOf>
      <rdfs:Class rdf:about="https://takin.solutions/ontologies/CRMcpr/CC5_Formulation"/>
    </rdfs:subClassOf>
  </rdfs:Class>
  <rdfs:Class rdf:about="https://takin.solutions/ontologies/CRMcpr/CC2_Realization">
    <skos:notation rdf:datatype="http://www.w3.org/2001/XMLSchema#string">CC2</skos:notation>
    <rdfs:comment xml:lang="en" rdf:datatype="http://www.w3.org/2001/XMLSchema#string">This class comprises the event of the instantiated realization of a planned artistic concept (CC20 Oeuvre), into an objective, concretized form (material and / or informational). This activity follows plans and projections delivered from one of more creative processes, such as CC14 Programme Conception, CC15 Design Conception and CC16 Realization Planning. Each of these is capable of delivering one or more outputs in the form of instances of CC5 Formulations which can be used by an instance of CC2 Realization to attempt to bring into existence the aimed for artistic object (E22 Human-made Object and/or E73 Information Object).</rdfs:comment>
    <rdfs:label xml:lang="en">Realization</rdfs:label>
    <rdfs:subClassOf>
      <rdfs:Class rdf:about="http://www.cidoc-crm.org/cidoc-crm/E65_Creation"/>
    </rdfs:subClassOf>
    <rdfs:subClassOf>
      <rdfs:Class rdf:about="http://www.cidoc-crm.org/cidoc-crm/E12_Production"/>
    </rdfs:subClassOf>
  </rdfs:Class>
  <rdfs:Class rdf:about="https://takin.solutions/ontologies/CRMcpr/CC3_Realization_Concept">
    <skos:notation rdf:datatype="http://www.w3.org/2001/XMLSchema#string">CC3</skos:notation>
    <rdfs:comment xml:lang="en" rdf:datatype="http://www.w3.org/2001/XMLSchema#string">This class comprises combinations of concepts such as are found in planning documents, including BIM, details, drawings, sketches, diagrams, blueprints, descriptions, 3D representations etc. which altogether aim to describe an approach for realizing an artistic concept. The instance of CC3 Realization Concept is a complex set of ideas that is proposed as the intellectual response to a certain projected CC13 Design Concept, which has itself typically been expressed in a number of instances of CC1 Model. An instance of CC3 Realization Concept is the overall approach for how to interpret the latter into a plan for the design’s physical realization or materialization (CC2 Realization). An instance of CC3 Realization Concept is typically elaborated by an actor acting as the “Maitrise d’Oeuvre” through different planning documents (instances of CC4 Realization Plan) that represent particular aspects of the overall plan. In the normal case, one of these proposals will be selected (CC19 Assessment)  as satisfying the CC13 Design Concept expressed in some particular set of instances of CC1 Model and will serve as the instance of CC4 Realization Plan that expresses the proposed CC3 Realization Concept.   The substance of CC3 Realization Concept is ideas; with regards to realizing objects into reality, the ideas proposed typically deal with the planning of the execution of a CC1 Model into a physical object, while taking into account various real-world constraints regarding the organization of the events necessary to bring this end about (CC12 Event Trigger Template). An instance of CC3 Realization Concept is complex by nature as it interacts with the set of constraints expressed in one or more instances of CC1 Model that detail the conceptual and physical aspects of the spatial projection selected as expressing the CC13 Design Concept.
The specific functionality of this class is to indicate the sets of concepts generated in order to plan the execution of an act of artistic realization of some object.</rdfs:comment>
    <rdfs:label xml:lang="en">Realization Concept</rdfs:label>
    <rdfs:subClassOf>
      <rdfs:Class rdf:about="http://iflastandards.info/ns/fr/frbr/frbroo/F15_Complex_Work"/>
    </rdfs:subClassOf>
  </rdfs:Class>
  <rdfs:Class rdf:about="https://takin.solutions/ontologies/CRMcpr/CC4_Realization_Plan">
    <skos:notation rdf:datatype="http://www.w3.org/2001/XMLSchema#string">CC4</skos:notation>
    <rdfs:comment xml:lang="en" rdf:datatype="http://www.w3.org/2001/XMLSchema#string">This class comprises the particularly expressed, immaterial, intellectual content of objects created during CC16 Realization Planning activities, in order to express and represent aspects of a projected CC2 Realization to be undertaken and its outcome. The propositional content contained in an instance of CC4 Realization Plan provides information regarding some aspect of an overall concept for a CC3 Realization Concept and can be used to understand the intent of the one who drafted the plan. Instances of this class are information objects produced as the result of realization planning processes (instances of F28 Expression Creation) undertaken in relation to the goals of an instance of an overall CC16 Realization Planning activity which, in turn, aims to comply with the specifications of an instance of CC1 Model. An instance of CC4 Realization Plan represents, in whole or in part, the propositional content of the instance of CC3 Realization Concept.</rdfs:comment>
    <rdfs:label xml:lang="en">Realization Plan</rdfs:label>
    <rdfs:subClassOf>
      <rdfs:Class rdf:about="https://takin.solutions/ontologies/CRMcpr/CC5_Formulation"/>
    </rdfs:subClassOf>
  </rdfs:Class>
  <rdfs:Class rdf:about="https://takin.solutions/ontologies/CRMcpr/CC5_Formulation">
    <skos:notation rdf:datatype="http://www.w3.org/2001/XMLSchema#string">CC5</skos:notation>
    <rdfs:comment xml:lang="en" rdf:datatype="http://www.w3.org/2001/XMLSchema#string">This class comprises the particularly expressed, immaterial, intellectual content of objects generated during creative conception activities which project certain potential events and objects into the world. The propositional content contained in a formulation provides information which represents particular creative concepts proposed for a certain project and which may provide information pertaining to a projected generated object and the manner of its CC2 Realization. Instances of this class are information objects arising through an activity of F28 Expression Creation, undertaken in relation to the goals of an instance of CC9 Oeuvre Conception, aiming towards realizing a creative idea. An instance of CC5 Formulation represents, in whole or in part, the propositional content of the instance of CC20 Oeuvre.</rdfs:comment>
    <rdfs:label xml:lang="en">Formulation</rdfs:label>
    <rdfs:subClassOf>
      <rdfs:Class rdf:about="http://www.cidoc-crm.org/cidoc-crm/E29_Design_or_Procedure"/>
    </rdfs:subClassOf>
    <rdfs:subClassOf>
      <rdfs:Class rdf:about="http://iflastandards.info/ns/fr/frbr/frbroo/F2_Expression"/>
    </rdfs:subClassOf>
  </rdfs:Class>
  <rdfs:Class rdf:about="https://takin.solutions/ontologies/CRMcpr/CC6_Programme">
    <skos:notation rdf:datatype="http://www.w3.org/2001/XMLSchema#string">CC6</skos:notation>
    <rdfs:comment xml:lang="en" rdf:datatype="http://www.w3.org/2001/XMLSchema#string">This class comprises the particularly expressed, immaterial, intellectual content of objects created during the creative programmation phase in order to express and represent CC17 Projective Requirements for a particular overall artistic project. This class comprises instances of information objects expressing projective requirements, wishes and needs for some CC20 Oeuvre in a formalized manner. A finalized, accepted CC6 Programme provides an expression of the requirements that will be employed to guide and constrain an eventual CC13 Design Concept. An instance of CC6 Programme comes into existence from an activity of expression creation (instance of F28 Expression Creation) and aims to represent, in whole or in part, the propositional content of the instance of CC17 Projective Requirements. </rdfs:comment>
    <rdfs:label xml:lang="en">Programme</rdfs:label>
    <rdfs:subClassOf>
      <rdfs:Class rdf:about="https://takin.solutions/ontologies/CRMcpr/CC5_Formulation"/>
    </rdfs:subClassOf>
  </rdfs:Class>
  <rdfs:Class rdf:about="https://takin.solutions/ontologies/CRMcpr/CC9_Oeuvre_Conception">
    <skos:notation rdf:datatype="http://www.w3.org/2001/XMLSchema#string">CC9</skos:notation>
    <rdfs:comment xml:lang="en" rdf:datatype="http://www.w3.org/2001/XMLSchema#string">This class comprises the evolution of a set of activities that aim towards the common intent of realizing a creative work in a broad sense. The coming into existence of an instance of CC9 Oeuvre Conception marks the initiation of an instance of CC20 Oeuvre. The latter intellectually gathers together the ideas and formulations contained in the various subworks (CC17 Projective Requirements, CC13 Design Concept, CC3 Realization Concept) and their formal expressions (CC6 Programme, CC1 Model, CC4 Realization Plan) that serve the common goal of the work’s final realization (CC2 Realization). In a commercial sphere, this is frequently undertaken with the participation of a client team acting as a client or patron and an executing team acting as a designer or service provider. An instance of this class often comes into being alongside the assignment of two groups as holding the roles of client and realizer who are formally attributed statuses as such. An associated ‘witness’ of such a will motivates the documentation of an instance of this event. Where possible, then, instances of CC9 Oeuvre Conception should be associated to instances of ZE6 Social Status through the property ZP75i is context for which document the actors causally implicated in willing the existence of the oeuvre and the roles that they play respectively, especially via their playing the role of client or patron / design or service provider. The instance of CC9 Oeuvre Conception is considered to be on-going and to encompass the sub-activities undertaken towards the realization of the main goal as long as the two parties continue to pursue this aim.</rdfs:comment>
    <rdfs:label xml:lang="en">Oeuvre Conception</rdfs:label>
    <rdfs:subClassOf>
      <rdfs:Class rdf:about="http://iflastandards.info/ns/fr/frbr/frbroo/F27_Work_Conception"/>
    </rdfs:subClassOf>
  </rdfs:Class>
  <rdfs:Class rdf:about="https://takin.solutions/ontologies/CRMcpr/CC11_Object_Trigger_Template">
    <skos:notation rdf:datatype="http://www.w3.org/2001/XMLSchema#string">CC11</skos:notation>
    <rdfs:comment xml:lang="en" rdf:datatype="http://www.w3.org/2001/XMLSchema#string">This class comprises specifications of projected artistic and architectural objects that detail constraints, specified as desired or necessary, that the projected object should comply with, according to a documented instance of CC5 Formulation. The function of CC11 Object Trigger Template is to allow the specification of qualities which the realized object should have such as dimension, material, function etc. The qualities specified here should be considered to stand as valid constraints to downstream and potentially upstream creative activities (CC14 Programme Conception, CC15 Design Conception, CC16 Realization Planning) within the context of an ongoing CC9 Oeuvre Conception, which can be used as to check conformity between desired and delivered outcomes ranging across realized plans (CC6 Programme, CC1 Model and CC4 Realization Plan) as well as the artistic object (E22 Human-made Object and/or E73 Information Object) finally generated through an act of CC2 Realization. 
For the documentation of the details of the constraints on the projected creation activity of a physical object (E22 Human-made Object), an associated instance of CC12 Event Trigger Template should be instantiated and connected through the property cp14i is stipulated object outcome.</rdfs:comment>
    <rdfs:label xml:lang="en">Object Trigger Template</rdfs:label>
    <rdfs:subClassOf>
      <rdfs:Class rdf:about="http://www.cidoc-crm.org/cidoc-crm/E89_Propositional_Object"/>
    </rdfs:subClassOf>
  </rdfs:Class>
  <rdfs:Class rdf:about="https://takin.solutions/ontologies/CRMcpr/CC12_Event_Trigger_Template">
    <skos:notation rdf:datatype="http://www.w3.org/2001/XMLSchema#string">CC12</skos:notation>
    <rdfs:comment xml:lang="en" rdf:datatype="http://www.w3.org/2001/XMLSchema#string">This class comprises specifications of projected creative activities towards the CC2 Realization of a creative work. It details guidelines and constraints that downstream and upstream creative activities should comply with, according to a documented instance of CC5 Formulation. The specified constraints can be instantiated on the level of kinds of processes, items or qualities and quantities involved in the action. The qualities specified here should be considered to stand as valid constraints on downstream and potentially upstream creative activities (CC14 Programme Conception, CC15 Design Conception, CC16 Realization Planning) within the context of an ongoing CC9 Oeuvre, which can be used as a check of conformity between desired and delivered outcomes ranging across instances of CC5 Formulation subtypes (i.e., CC6 Programme, CC1 Model and CC4 Realization Plan) as well as the act of CC2 Realization itself, unless a newer instance of CC5 Formulation is created to supersede.
An instance of an expected kind of outcome in terms of object, e.g. design or building, is typically implied in most instances of CC12 Event Trigger Template and should be documented via an instance of CC11 Object Trigger Template. </rdfs:comment>
    <rdfs:label xml:lang="en">Event Trigger Template</rdfs:label>
    <rdfs:subClassOf>
      <rdfs:Class rdf:about="http://www.cidoc-crm.org/cidoc-crm/E89_Propositional_Object"/>
    </rdfs:subClassOf>
  </rdfs:Class>
  <rdfs:Class rdf:about="https://takin.solutions/ontologies/CRMcpr/CC13_Design_Concept">
    <skos:notation rdf:datatype="http://www.w3.org/2001/XMLSchema#string">CC13</skos:notation>
    <rdfs:comment xml:lang="en" rdf:datatype="http://www.w3.org/2001/XMLSchema#string">This class comprises combinations of concepts found in creative expressions, such as drawings, sketches, diagrams, plans, descriptions, 3D representations etc, which together form an overall concept for a design. An instance of CC13 Design Concept is a complex set of ideas that is proposed as the intellectual response to a certain, projected creative aim, that may be documented as an instance of CC6 Programme, expressing the latter as particular creative design proposals. The CC13 Design Concept is typically elaborated by an actor in the role of ‘Maitrise d’Oeuvre’ through different design documents (instances of CC1 Model) that represent various aspects of the overall idea. The substance of CC13 Design Concept is ideas. 
An instance of CC13 Design Concept is complex by nature as it interacts with the set of requirements typically expressed in an instance of CC6 Programme, which concretizes the requirements set out by an instance of CC17 Projective Requirements. It is articulated through various documents expressing different collective proposals that will go through processes of selection and filtering. In the normal case, one of these proposals will be selected as satisfying the CC17 Projective Requirements expressed in a CC6 Programme and serve as the accepted instance(s) of CC1 Model that expresses the final CC13 Design Concept.</rdfs:comment>
    <rdfs:label xml:lang="en">Design Concept</rdfs:label>
    <rdfs:subClassOf>
      <rdfs:Class rdf:about="http://iflastandards.info/ns/fr/frbr/frbroo/F15_Complex_Work"/>
    </rdfs:subClassOf>
  </rdfs:Class>
  <rdfs:Class rdf:about="https://takin.solutions/ontologies/CRMcpr/CC14_Programme_Conception">
    <skos:notation rdf:datatype="http://www.w3.org/2001/XMLSchema#string">CC14</skos:notation>
    <rdfs:comment xml:lang="en" rdf:datatype="http://www.w3.org/2001/XMLSchema#string">This class comprises the beginning of the evolution of a set of activities that aim towards the formulation of user or client’s (e.g.: a designated “Maîtrise d'Ouvrage”) needs, wishes and requirements for a projected CC20 Oeuvre. The substance of programming is intentional activity towards generated CC17 Projective Requirements that will typically be formally specified and approved in a requirements document, an instance of CC6 Programme. The instance of CC14 Programme Conception begins when the client starts to formulate their needs, with or without external party participation of the eventually designated realizing party (e.g., a designated ‘Maîtrise d'Oeuvre’).</rdfs:comment>
    <rdfs:label xml:lang="en">Programme Conception</rdfs:label>
    <rdfs:subClassOf>
      <rdfs:Class rdf:about="http://iflastandards.info/ns/fr/frbr/frbroo/F27_Work_Conception"/>
    </rdfs:subClassOf>
  </rdfs:Class>
  <rdfs:Class rdf:about="https://takin.solutions/ontologies/CRMcpr/CC15_Design_Conception">
    <skos:notation rdf:datatype="http://www.w3.org/2001/XMLSchema#string">CC15</skos:notation>
    <rdfs:comment xml:lang="en" rdf:datatype="http://www.w3.org/2001/XMLSchema#string">This class comprises the beginning of the evolution of a set of activities that aim towards the formulation of a creative design concept (CC13), realized in one or more instances of CC1 Model, that usually respond to an instance of CC17 Projective Requirements formulated for a projected creative work (CC20). The substance of design conception is intentional activity towards the formalization of a proposal detailing a (series of) model(s) (CC1) aiming to satisfy the initiating client’s requirements expressed in a formal programme (CC6). The instance of design conception begins when the actor charged with realizing the creative work (e.g.: the designated ‘Maîtrise d'Oeuvre’) starts the activities to formulate a design proposal, with or without an external party participating, which may or may not include the designated ‘Maîtrise d'Ouvrage’.</rdfs:comment>
    <rdfs:label xml:lang="en">Design Conception</rdfs:label>
    <rdfs:subClassOf>
      <rdfs:Class rdf:about="http://iflastandards.info/ns/fr/frbr/frbroo/F27_Work_Conception"/>
    </rdfs:subClassOf>
  </rdfs:Class>
  <rdfs:Class rdf:about="https://takin.solutions/ontologies/CRMcpr/CC16_Realization_Planning">
    <skos:notation rdf:datatype="http://www.w3.org/2001/XMLSchema#string">CC16</skos:notation>
    <rdfs:comment xml:lang="en" rdf:datatype="http://www.w3.org/2001/XMLSchema#string">This class comprises the beginning of the evolution of a set of activities that aim towards the articulation of a CC3 Realization Concept, concretized in one or more CC4 Realization Plans, which aim to accurately incorporate a specific set of design documents (instances of CC1 Model) into a plan to realize a creative idea, typically as a physical work (E22 Human-made Object). The instance of this event begins when an actor, such as that designated ‘Maîtrise d'Oeuvre’, starts the activities of formulating the plan towards realization, with or without an external party participating, which may or may not include the ‘Maîtrise d'Ouvrage’. </rdfs:comment>
    <rdfs:label xml:lang="en">Realization Planning</rdfs:label>
    <rdfs:subClassOf>
      <rdfs:Class rdf:about="http://iflastandards.info/ns/fr/frbr/frbroo/F27_Work_Conception"/>
    </rdfs:subClassOf>
  </rdfs:Class>
  <rdfs:Class rdf:about="https://takin.solutions/ontologies/CRMcpr/CC17_Projective_Requirements">
    <skos:notation rdf:datatype="http://www.w3.org/2001/XMLSchema#string">CC17</skos:notation>
    <rdfs:comment xml:lang="en" rdf:datatype="http://www.w3.org/2001/XMLSchema#string">This class comprises distinct concepts or combinations of concepts embodying the aim, will and/or desire of an actor with regards to a particular projected CC20 Oeuvre. The instance of CC17 Projective Requirements is elicited from an actor either by him/herself or, more usually, with others, in order to express it in some concrete, documented form which will be used to guide the activities of a CC15 Design Conception. The substance of an instance of CC17 Projective Requirements is ideas in the sense of an articulated will, aim and desire with regards to a projected outcome, which is usually elaborated and reformulated over time in different iterations and derivations of the initial will, and finally realized in one or more CC6 Programmes, to be adopted as a guide in the design phase.</rdfs:comment>
    <rdfs:label xml:lang="en">Projective Requirements</rdfs:label>
    <rdfs:subClassOf>
      <rdfs:Class rdf:about="http://iflastandards.info/ns/fr/frbr/frbroo/F15_Complex_Work"/>
    </rdfs:subClassOf>
  </rdfs:Class>
  <rdfs:Class rdf:about="https://takin.solutions/ontologies/CRMcpr/CC19_Assessment">
    <skos:notation rdf:datatype="http://www.w3.org/2001/XMLSchema#string">CC19</skos:notation>
    <rdfs:comment xml:lang="en" rdf:datatype="http://www.w3.org/2001/XMLSchema#string">This class comprises acts of evaluation of an instance of E73 Information Object against an implicit or explicit standard by some actor. An instance of CC19 Assessment is undertaken in order to provide some form of feedback and evaluation on the assessed instance of E73 Information Object in the form of a categorical assessment, a reviewed information object or both. An act of assessment may result in the assignment of an evaluative categorical rank to the assessed conceptual pattern. An act of assessment may also result in a revised version of the assessed instance of E73 Information Object being produced by the assessor. The newly resultant assessed instance of E73 Information Object may include additions, deletions, modifications and commentaries relative to the original target of assessment. The resultant instance information object is, then, considered to incorporate elements of the original E73 Information Object. The edge cases of an act of assessment are the rejection or acceptance of the assessed E73 Information Object. In the case of rejection, the assessed information object has been categorized as a failure by the assessing actor, potentially terminating a direction of creation. In the case of approval, the assessed information object is considered to have been categorized as accepted in toto qua information object by the assessor, relative to the standard of evaluation. Acts of assessment are considered to generate and be generated by instances of F28 Expression Creation in a cycle that typically aims towards achieving an acceptance evaluation. Within the context of a cycle of creative processes, an act of assessment resulting in an assignment of approval typically indicates that the assessor considers the main idea and all relevant additional parameters of judgement with regards to the formulation of the object to be satisfactory and to express the instance of F15 Complex Work which it was formulated to materialize.  </rdfs:comment>
    <rdfs:label xml:lang="en">Assessment</rdfs:label>
    <rdfs:subClassOf>
      <rdfs:Class rdf:about="http://www.cidoc-crm.org/cidoc-crm/E17_Type_Assignment"/>
    </rdfs:subClassOf>
    <rdfs:subClassOf>
      <rdfs:Class rdf:about="http://www.cidoc-crm.org/cidoc-crm/E65_Creation"/>
    </rdfs:subClassOf>
  </rdfs:Class>
  <rdfs:Class rdf:about="https://takin.solutions/ontologies/CRMcpr/CC20_Oeuvre">
    <skos:notation rdf:datatype="http://www.w3.org/2001/XMLSchema#string">CC20</skos:notation>
    <rdfs:comment xml:lang="en" rdf:datatype="http://www.w3.org/2001/XMLSchema#string">This class comprises combinations of concepts that together represent a recognizable novel intellectual content that is intended to be realized into a particular physical or conceptual form. The substance of an instance of this class is its unique set of ideas. An instance of this class is complex in that it is typically composed of a set of other ideas which together form its content. An instance of CC20 Oeuvre is typically formed of member works consisting of a CC17 Project Requirement, CC13 Design Concept and a CC4 Realization Plan. Together these works are progressively realized in order to be able to bring into existence a particular creation, physical or intellectual, through a CC2 Realization act. An instance of this class comes to be through its initiation by an activity of creation (CC9 Oeuvre Conception) which, in turn, entails the willing of the realization of this idea by one or more parties acting as patrons and service providers in turn. The substance of CC20 Oeuvre is ideas. 
An instance of CC20 Oeuvre represents the most abstract level of a creative intellectual project, and gathers together all the particular ideas created towards its expression into a larger whole. CC20 Oeuvre stands apart from any individual physical or intellectual creation undertaken in the elaboration of a creative idea and stands for the idea itself. The documentation of an instance of CC20 Oeuvre thus allows both for the richer elaboration of the elements that lead to an eventual physical or intellectual instantiation of the idea through tracing the individual processes and components leading to a final as well as supporting the possibility to document partially realized or mostly unrealized creative projects.  </rdfs:comment>
    <rdfs:label xml:lang="en">Oeuvre</rdfs:label>
    <rdfs:subClassOf>
      <rdfs:Class rdf:about="http://iflastandards.info/ns/fr/frbr/frbroo/F15_Complex_Work"/>
    </rdfs:subClassOf>
  </rdfs:Class>
 
  <rdf:Property rdf:about="https://takin.solutions/ontologies/CRMcpr/CP4_projects">
    <rdfs:range rdf:resource="https://takin.solutions/ontologies/CRMcpr/CC12_Event_Trigger_Template"/>
    <rdfs:comment xml:lang="en">This property describes the relation between a CC5 Formulation and a projected event it plans for. Instances of CC5 Formulation may contain detailed, analytic information regarding how the plan formulates an intended event, or set of events, to occur, documenting also how and under what conditions a specific event can be said to have taken place and achieved according to a set of agreed terms. By instantiating this property, an activity plan can be connected to the analytic information it details for the projected manner of execution of the event that it foresees.</rdfs:comment>
    <rdfs:label xml:lang="en">projects</rdfs:label>
    <skos:notation rdf:datatype="http://www.w3.org/2001/XMLSchema#string">CP4</skos:notation>
    <rdfs:domain rdf:resource="https://takin.solutions/ontologies/CRMcpr/CC5_Formulation"/>
  </rdf:Property>
  <rdf:Property rdf:about="https://takin.solutions/ontologies/CRMcpr/CP5_stipulates_type_of_object_outcome">
    <rdfs:range rdf:resource="http://www.cidoc-crm.org/cidoc-crm/E55_Type"/>
    <rdfs:comment xml:lang="en">This property describes what type of object has been stipulated in a CC12 Event Trigger Template, as expected to be brought into existence through the event it projects. The form of stipulation is categorical, specifying a kind of object to be produced but not its particular features.</rdfs:comment>
    <rdfs:label xml:lang="en">stipulates type of object outcome</rdfs:label>
    <skos:notation rdf:datatype="http://www.w3.org/2001/XMLSchema#string">CP5</skos:notation>
    <rdfs:domain rdf:resource="https://takin.solutions/ontologies/CRMcpr/CC12_Event_Trigger_Template"/>
  </rdf:Property>
  <rdf:Property rdf:about="https://takin.solutions/ontologies/CRMcpr/CP6_stipulates_event_type">
    <rdfs:range rdf:resource="http://www.cidoc-crm.org/cidoc-crm/E55_Type"/>
    <rdfs:comment xml:lang="en">This property describes what form of activity the projected event is expected to consist in, stipulating its basic nature such as: production, communication, design.</rdfs:comment>
    <rdfs:label xml:lang="en">stipulates event type</rdfs:label>
    <skos:notation rdf:datatype="http://www.w3.org/2001/XMLSchema#string">CP6</skos:notation>
    <rdfs:domain rdf:resource="https://takin.solutions/ontologies/CRMcpr/CC12_Event_Trigger_Template"/>
  </rdf:Property>
  <rdf:Property rdf:about="https://takin.solutions/ontologies/CRMcpr/CP7_stipulates_actor_type">
    <rdfs:range rdf:resource="http://www.cidoc-crm.org/cidoc-crm/E55_Type"/>
    <rdfs:comment xml:lang="en">This property describes the kind(s) of actor that a projected activity is foreseen to involve. It thus allows the description of kinds of participants in the foreseen event at the categorical level. A plan may, thus, call for a certain type of professional to be involved, a certain category of individual etc.</rdfs:comment>
    <rdfs:label xml:lang="en">stipulates actor type</rdfs:label>
    <skos:notation rdf:datatype="http://www.w3.org/2001/XMLSchema#string">CP7</skos:notation>
    <rdfs:domain rdf:resource="https://takin.solutions/ontologies/CRMcpr/CC12_Event_Trigger_Template"/>
  </rdf:Property>
  <rdf:Property rdf:about="https://takin.solutions/ontologies/CRMcpr/CP8_stipulates_place">
    <rdfs:range rdf:resource="http://www.cidoc-crm.org/cidoc-crm/E53_Place"/>
    <rdfs:comment xml:lang="en">This property describes the expected, real-world place where the projected event is supposed to occur.</rdfs:comment>
    <rdfs:label xml:lang="en">stipulates place</rdfs:label>
    <skos:notation rdf:datatype="http://www.w3.org/2001/XMLSchema#string">CP8</skos:notation>
    <rdfs:domain rdf:resource="https://takin.solutions/ontologies/CRMcpr/CC12_Event_Trigger_Template"/>
  </rdf:Property>
  <rdf:Property rdf:about="https://takin.solutions/ontologies/CRMcpr/CP9_stipulates_time-span">
    <rdfs:range rdf:resource="http://www.cidoc-crm.org/cidoc-crm/E52_Time-Span"/>
    <rdfs:comment xml:lang="en">This property describes the expected time-span within which the projected event is supposed to occur.</rdfs:comment>
    <rdfs:label xml:lang="en">stipulates time-span</rdfs:label>
    <skos:notation rdf:datatype="http://www.w3.org/2001/XMLSchema#string">CP9</skos:notation>
    <rdfs:domain rdf:resource="https://takin.solutions/ontologies/CRMcpr/CC12_Event_Trigger_Template"/>
  </rdf:Property>
  <rdf:Property rdf:about="https://takin.solutions/ontologies/CRMcpr/CP10_stipulates_actor">
    <rdfs:range rdf:resource="http://www.cidoc-crm.org/cidoc-crm/E39_Actor"/>
    <rdfs:comment xml:lang="en">This property describes instances of particular individuals persons or groups that are expected to participate within the projected event.</rdfs:comment>
    <rdfs:label xml:lang="en">stipulates actor</rdfs:label>
    <skos:notation rdf:datatype="http://www.w3.org/2001/XMLSchema#string">CP10</skos:notation>
    <rdfs:domain rdf:resource="https://takin.solutions/ontologies/CRMcpr/CC12_Event_Trigger_Template"/>
  </rdf:Property>
  <rdf:Property rdf:about="https://takin.solutions/ontologies/CRMcpr/CP11_stipulates_equipment">
    <rdfs:range rdf:resource="http://www.cidoc-crm.org/cidoc-crm/E18_Physical_Thing"/>
    <rdfs:comment xml:lang="en">This property describes instances of equipment (E18) that are stipulated as expected to be used in the carrying out of the projected event.</rdfs:comment>
    <rdfs:label xml:lang="en">stipulates equipment</rdfs:label>
    <skos:notation rdf:datatype="http://www.w3.org/2001/XMLSchema#string">CP11</skos:notation>
    <rdfs:domain rdf:resource="https://takin.solutions/ontologies/CRMcpr/CC12_Event_Trigger_Template"/>
  </rdf:Property>
  <rdf:Property rdf:about="https://takin.solutions/ontologies/CRMcpr/CP12_stipulates_particular_method">
    <rdfs:range rdf:resource="http://www.cidoc-crm.org/cidoc-crm/E29_Design_or_Procedure"/>
    <rdfs:comment xml:lang="en">This property describes instances of design or procedures that are stipulated to be followed in the carrying out of the projected event.</rdfs:comment>
    <rdfs:label xml:lang="en">stipulates particular method</rdfs:label>
    <skos:notation rdf:datatype="http://www.w3.org/2001/XMLSchema#string">CP12</skos:notation>
    <rdfs:domain rdf:resource="https://takin.solutions/ontologies/CRMcpr/CC12_Event_Trigger_Template"/>
  </rdf:Property>
  <rdf:Property rdf:about="https://takin.solutions/ontologies/CRMcpr/CP13_stipulates_specific_budget">
    <rdfs:range rdf:resource="http://www.cidoc-crm.org/cidoc-crm/E54_Dimension"/>
    <rdfs:comment xml:lang="en">This property describes the budget that is stipulated as a constraint to the carrying out of the projected event.</rdfs:comment>
    <rdfs:label xml:lang="en">stipulates specific budget</rdfs:label>
    <skos:notation rdf:datatype="http://www.w3.org/2001/XMLSchema#string">CP13</skos:notation>
    <rdfs:domain rdf:resource="https://takin.solutions/ontologies/CRMcpr/CC12_Event_Trigger_Template"/>
  </rdf:Property>
  <rdf:Property rdf:about="https://takin.solutions/ontologies/CRMcpr/CP14_stipulates_object_outcome">
    <rdfs:range rdf:resource="https://takin.solutions/ontologies/CRMcpr/CC11_Object_Trigger_Template"/>
    <rdfs:comment xml:lang="en">This property relates an instance of Event Trigger Template to an instance of Objecter Trigger Template that is specified to be an outcome of the projected event. </rdfs:comment>
    <rdfs:label xml:lang="en">stipulates object outcome</rdfs:label>
    <skos:notation rdf:datatype="http://www.w3.org/2001/XMLSchema#string">CP14</skos:notation>
    <rdfs:domain rdf:resource="https://takin.solutions/ontologies/CRMcpr/CC12_Event_Trigger_Template"/>
  </rdf:Property>
  <rdf:Property rdf:about="https://takin.solutions/ontologies/CRMcpr/CP15_stipulates_sub-event">
    <rdfs:range rdf:resource="https://takin.solutions/ontologies/CRMcpr/CC12_Event_Trigger_Template"/>
    <rdfs:comment xml:lang="en">This property enables the documentation of planned sub-events stipulated as part of an overall projected event. It is used to link an instance of Event Trigger Template to another instance of this class which would be an element of its own execution. The intention of this property is to enable the modelling of the projection of a complex event with sub-elements.</rdfs:comment>
    <rdfs:label xml:lang="en">stipulates sub-event</rdfs:label>
    <skos:notation rdf:datatype="http://www.w3.org/2001/XMLSchema#string">CP15</skos:notation>
    <rdfs:domain rdf:resource="https://takin.solutions/ontologies/CRMcpr/CC12_Event_Trigger_Template"/>
  </rdf:Property>
  <rdf:Property rdf:about="https://takin.solutions/ontologies/CRMcpr/CP16_stipulates_material">
    <rdfs:range rdf:resource="http://www.cidoc-crm.org/cidoc-crm/E57_Material"/>
    <rdfs:comment xml:lang="en">This property describes the material of which the projected object is expected to be comprised.</rdfs:comment>
    <rdfs:label xml:lang="en">stipulates material</rdfs:label>
    <skos:notation rdf:datatype="http://www.w3.org/2001/XMLSchema#string">CP16</skos:notation>
    <rdfs:domain rdf:resource="https://takin.solutions/ontologies/CRMcpr/CC11_Object_Trigger_Template"/>
  </rdf:Property>
  <rdf:Property rdf:about="https://takin.solutions/ontologies/CRMcpr/CP17_stipulates_site">
    <rdfs:range rdf:resource="http://www.cidoc-crm.org/cidoc-crm/E27_Site"/>
    <rdfs:comment xml:lang="en">This property describes a particular real world site at which the projected object is expected to be installed or placed.</rdfs:comment>
    <rdfs:label xml:lang="en">stipulates site</rdfs:label>
    <skos:notation rdf:datatype="http://www.w3.org/2001/XMLSchema#string">CP17</skos:notation>
    <rdfs:domain rdf:resource="https://takin.solutions/ontologies/CRMcpr/CC11_Object_Trigger_Template"/>
  </rdf:Property>
  <rdf:Property rdf:about="https://takin.solutions/ontologies/CRMcpr/CP18_stipulates_dimension">
    <rdfs:range rdf:resource="http://www.cidoc-crm.org/cidoc-crm/E54_Dimension"/>
    <rdfs:comment xml:lang="en">This property describes the expected dimensions of the projected object.</rdfs:comment>
    <rdfs:label xml:lang="en">stipulates dimension</rdfs:label>
    <skos:notation rdf:datatype="http://www.w3.org/2001/XMLSchema#string">CP18</skos:notation>
    <rdfs:domain rdf:resource="https://takin.solutions/ontologies/CRMcpr/CC11_Object_Trigger_Template"/>
  </rdf:Property>
  <rdf:Property rdf:about="https://takin.solutions/ontologies/CRMcpr/CP19_stipulates_function">
    <rdfs:range rdf:resource="http://www.cidoc-crm.org/cidoc-crm/E55_Type"/>
    <rdfs:comment xml:lang="en">This property describes the expected function of the projected object.</rdfs:comment>
    <rdfs:label xml:lang="en">stipulates function</rdfs:label>
    <skos:notation rdf:datatype="http://www.w3.org/2001/XMLSchema#string">CP19</skos:notation>
    <rdfs:domain rdf:resource="https://takin.solutions/ontologies/CRMcpr/CC11_Object_Trigger_Template"/>
  </rdf:Property>
  <rdf:Property rdf:about="https://takin.solutions/ontologies/CRMcpr/CP20_stipulates_reference">
    <rdfs:range rdf:resource="http://www.cidoc-crm.org/cidoc-crm/E73_Information_Object"/>
    <rdfs:comment xml:lang="en">This property associates an instance of Object Trigger Template with an Information Object which is to be used as a reference in the making of the projected object. The end result should show similarity to the referenced object</rdfs:comment>
    <rdfs:label xml:lang="en">stipulates reference</rdfs:label>
    <skos:notation rdf:datatype="http://www.w3.org/2001/XMLSchema#string">CP20</skos:notation>
    <rdfs:domain rdf:resource="https://takin.solutions/ontologies/CRMcpr/CC11_Object_Trigger_Template"/>
  </rdf:Property>
  <rdf:Property rdf:about="https://takin.solutions/ontologies/CRMcpr/CP21_stipulates_part">
    <rdfs:range rdf:resource="https://takin.solutions/ontologies/CRMcpr/CC11_Object_Trigger_Template"/>
    <rdfs:comment xml:lang="en">This property enables the documentation of expected parts of a planned object and the particular features of those parts.</rdfs:comment>
    <rdfs:label xml:lang="en">stipulates part</rdfs:label>
    <skos:notation rdf:datatype="http://www.w3.org/2001/XMLSchema#string">CP21</skos:notation>
    <rdfs:domain rdf:resource="https://takin.solutions/ontologies/CRMcpr/CC11_Object_Trigger_Template"/>
  </rdf:Property>
  <rdf:Property rdf:about="https://takin.solutions/ontologies/CRMcpr/CP22_assessed">
    <rdfs:range rdf:resource="http://www.cidoc-crm.org/cidoc-crm/E73_Information_Object"/>
    <rdfs:comment xml:lang="en">This property indicates that an assessment activity was carried out on an instance of information object.</rdfs:comment>
    <rdfs:label xml:lang="en">assessed</rdfs:label>
    <skos:notation rdf:datatype="http://www.w3.org/2001/XMLSchema#string">CP22</skos:notation>
    <rdfs:domain rdf:resource="https://takin.solutions/ontologies/CRMcpr/CC19_Assessment"/>
  </rdf:Property>
  <rdf:Property rdf:about="https://takin.solutions/ontologies/CRMcpr/CP24_produced_revision">
    <rdfs:range rdf:resource="http://www.cidoc-crm.org/cidoc-crm/E73_Information_Object"/>
    <rdfs:comment xml:lang="en">This property indicates that a new information object was created out of an assessment activity. The generated instance of information object will incorporate the assessed information object but may have added, removed, or modified its content as part of the assessment activity.</rdfs:comment>
    <rdfs:label xml:lang="en">produced revision</rdfs:label>
    <skos:notation rdf:datatype="http://www.w3.org/2001/XMLSchema#string">CP24</skos:notation>
    <rdfs:domain rdf:resource="https://takin.solutions/ontologies/CRMcpr/CC19_Assessment"/>
  </rdf:Property>
  <rdf:Property rdf:about="https://takin.solutions/ontologies/CRMcpr/CP25_concerns_extant_object">
    <rdfs:range rdf:resource="http://www.cidoc-crm.org/cidoc-crm/E18_Physical_Thing"/>
    <rdfs:comment xml:lang="en">This property describes instances of things that are the main object concerned in the realization of the projected new configuration of an extant object. The execution of the object template may result in modification or transformation of the object indicated by this property.</rdfs:comment>
    <rdfs:label xml:lang="en">concerns extant object</rdfs:label>
    <skos:notation rdf:datatype="http://www.w3.org/2001/XMLSchema#string">CP25</skos:notation>
    <rdfs:domain rdf:resource="https://takin.solutions/ontologies/CRMcpr/CC11_Object_Trigger_Template"/>
  </rdf:Property>

 <rdf:Property rdf:about="https://takin.solutions/ontologies/CRMcpr/CP4i_was_projected_by">
    <rdfs:domain rdf:resource="https://takin.solutions/ontologies/CRMcpr/CC12_Event_Trigger_Template"/>
    <rdfs:comment xml:lang="en">This property is the inverse of the forward property described in the scope note that follows. This property describes the relation between a CC5 Formulation and a projected event it plans for. Instances of CC5 Formulation may contain detailed, analytic information regarding how the plan formulates an intended event, or set of events, to occur, documenting also how and under what conditions a specific event can be said to have taken place and achieved according to a set of agreed terms. By instantiating this property, an activity plan can be connected to the analytic information it details for the projected manner of execution of the event that it foresees.</rdfs:comment>
    <rdfs:label xml:lang="en">was projected by</rdfs:label>
    <skos:notation rdf:datatype="http://www.w3.org/2001/XMLSchema#string">CP4i</skos:notation>
    <rdfs:range rdf:resource="https://takin.solutions/ontologies/CRMcpr/CC5_Formulation"/>
  </rdf:Property>
  <rdf:Property rdf:about="https://takin.solutions/ontologies/CRMcpr/CP5i_is_type_of_object_outcome_stipulated_by">
    <rdfs:domain rdf:resource="http://www.cidoc-crm.org/cidoc-crm/E55_Type"/>
    <rdfs:comment xml:lang="en">This property is the inverse of the forward property described in the scope note that follows. This property describes what type of object has been stipulated in a CC12 Event Trigger Template, as expected to be brought into existence through the event it projects. The form of stipulation is categorical, specifying a kind of object to be produced but not its particular features.</rdfs:comment>
    <rdfs:label xml:lang="en">is type of object outcome stipulated by</rdfs:label>
    <skos:notation rdf:datatype="http://www.w3.org/2001/XMLSchema#string">CP5i</skos:notation>
    <rdfs:range rdf:resource="https://takin.solutions/ontologies/CRMcpr/CC12_Event_Trigger_Template"/>
  </rdf:Property>
  <rdf:Property rdf:about="https://takin.solutions/ontologies/CRMcpr/CP6i_is_type_of_event_type_stipulated_by">
    <rdfs:domain rdf:resource="http://www.cidoc-crm.org/cidoc-crm/E55_Type"/>
    <rdfs:comment xml:lang="en">This property is the inverse of the forward property described in the scope note that follows. This property describes what form of activity the projected event is expected to consist in, stipulating its basic nature such as: production, communication, design.</rdfs:comment>
    <rdfs:label xml:lang="en">is type of event stipulated by</rdfs:label>
    <skos:notation rdf:datatype="http://www.w3.org/2001/XMLSchema#string">CP6i</skos:notation>
    <rdfs:range rdf:resource="https://takin.solutions/ontologies/CRMcpr/CC12_Event_Trigger_Template"/>
  </rdf:Property>
  <rdf:Property rdf:about="https://takin.solutions/ontologies/CRMcpr/CP7i_is_actor_type_stipulated_by">
    <rdfs:domain rdf:resource="http://www.cidoc-crm.org/cidoc-crm/E55_Type"/>
    <rdfs:comment xml:lang="en">This property is the inverse of the forward property described in the scope note that follows. This property describes the kind(s) of actor that a projected activity is foreseen to involve. It thus allows the description of kinds of participants in the foreseen event at the categorical level. A plan may, thus, call for a certain type of professional to be involved, a certain category of individual etc.</rdfs:comment>
    <rdfs:label xml:lang="en">is actor type stipulated by</rdfs:label>
    <skos:notation rdf:datatype="http://www.w3.org/2001/XMLSchema#string">CP7i</skos:notation>
    <rdfs:range rdf:resource="https://takin.solutions/ontologies/CRMcpr/CC12_Event_Trigger_Template"/>
  </rdf:Property>
  <rdf:Property rdf:about="https://takin.solutions/ontologies/CRMcpr/CP8i_is_place_stipulated_by">
    <rdfs:domain rdf:resource="http://www.cidoc-crm.org/cidoc-crm/E53_Place"/>
    <rdfs:comment xml:lang="en">This property is the inverse of the forward property described in the scope note that follows. This property describes the expected, real-world place where the projected event is supposed to occur.</rdfs:comment>
    <rdfs:label xml:lang="en">is place stipulated by</rdfs:label>
    <skos:notation rdf:datatype="http://www.w3.org/2001/XMLSchema#string">CP8i</skos:notation>
    <rdfs:range rdf:resource="https://takin.solutions/ontologies/CRMcpr/CC12_Event_Trigger_Template"/>
  </rdf:Property>
  <rdf:Property rdf:about="https://takin.solutions/ontologies/CRMcpr/CP9i_is_time-span_stipulated_by">
    <rdfs:domain rdf:resource="http://www.cidoc-crm.org/cidoc-crm/E52_Time-Span"/>
    <rdfs:comment xml:lang="en">This property is the inverse of the forward property described in the scope note that follows. This property describes the expected time-span within which the projected event is supposed to occur.</rdfs:comment>
    <rdfs:label xml:lang="en">is time-span stipulated by</rdfs:label>
    <skos:notation rdf:datatype="http://www.w3.org/2001/XMLSchema#string">CP9i</skos:notation>
    <rdfs:range rdf:resource="https://takin.solutions/ontologies/CRMcpr/CC12_Event_Trigger_Template"/>
  </rdf:Property>
  <rdf:Property rdf:about="https://takin.solutions/ontologies/CRMcpr/CP10i_is_actor_stipulated_by">
    <rdfs:domain rdf:resource="http://www.cidoc-crm.org/cidoc-crm/E39_Actor"/>
    <rdfs:comment xml:lang="en">This property is the inverse of the forward property described in the scope note that follows. This property describes instances of particular individuals persons or groups that are expected to participate within the projected event.</rdfs:comment>
    <rdfs:label xml:lang="en">is actor stipulated by</rdfs:label>
    <skos:notation rdf:datatype="http://www.w3.org/2001/XMLSchema#string">CP10i</skos:notation>
    <rdfs:range rdf:resource="https://takin.solutions/ontologies/CRMcpr/CC12_Event_Trigger_Template"/>
  </rdf:Property>
  <rdf:Property rdf:about="https://takin.solutions/ontologies/CRMcpr/CP11i_is_equipment_stipulated_by">
    <rdfs:domain rdf:resource="http://www.cidoc-crm.org/cidoc-crm/E18_Physical_Thing"/>
    <rdfs:comment xml:lang="en">This property is the inverse of the forward property described in the scope note that follows. This property describes instances of equipment (E18) that are stipulated as expected to be used in the carrying out of the projected event.</rdfs:comment>
    <rdfs:label xml:lang="en">is equipment stipulated by</rdfs:label>
    <skos:notation rdf:datatype="http://www.w3.org/2001/XMLSchema#string">CP11i</skos:notation>
    <rdfs:range rdf:resource="https://takin.solutions/ontologies/CRMcpr/CC12_Event_Trigger_Template"/>
  </rdf:Property>
  <rdf:Property rdf:about="https://takin.solutions/ontologies/CRMcpr/CP12i_is_particular_method_stipulated_by">
    <rdfs:domain rdf:resource="http://www.cidoc-crm.org/cidoc-crm/E29_Design_or_Procedure"/>
    <rdfs:comment xml:lang="en">This property is the inverse of the forward property described in the scope note that follows. This property describes instances of design or procedures that are stipulated to be followed in the carrying out of the projected event.</rdfs:comment>
    <rdfs:label xml:lang="en">is particular method stipulated by</rdfs:label>
    <skos:notation rdf:datatype="http://www.w3.org/2001/XMLSchema#string">CP12i</skos:notation>
    <rdfs:range rdf:resource="https://takin.solutions/ontologies/CRMcpr/CC12_Event_Trigger_Template"/>
  </rdf:Property>
  <rdf:Property rdf:about="https://takin.solutions/ontologies/CRMcpr/CP13i_is_budget_stipulated_by">
    <rdfs:domain rdf:resource="http://www.cidoc-crm.org/cidoc-crm/E54_Dimension"/>
    <rdfs:comment xml:lang="en">This property is the inverse of the forward property described in the scope note that follows. This property describes the budget that is stipulated as a constraint to the carrying out of the projected event.</rdfs:comment>
    <rdfs:label xml:lang="en">is budget stipulated by</rdfs:label>
    <skos:notation rdf:datatype="http://www.w3.org/2001/XMLSchema#string">CP13i</skos:notation>
    <rdfs:range rdf:resource="https://takin.solutions/ontologies/CRMcpr/CC12_Event_Trigger_Template"/>
  </rdf:Property>
  <rdf:Property rdf:about="https://takin.solutions/ontologies/CRMcpr/CP14i_is_object_outcome_stipulated_by">
    <rdfs:domain rdf:resource="https://takin.solutions/ontologies/CRMcpr/CC11_Object_Trigger_Template"/>
    <rdfs:comment xml:lang="en">This property is the inverse of the forward property described in the scope note that follows. This property relates an instance of Event Trigger Template to an instance of Objecter Trigger Template that is specified to be an outcome of the projected event. </rdfs:comment>
    <rdfs:label xml:lang="en">is object outcome stipulated by</rdfs:label>
    <skos:notation rdf:datatype="http://www.w3.org/2001/XMLSchema#string">CP14i</skos:notation>
    <rdfs:range rdf:resource="https://takin.solutions/ontologies/CRMcpr/CC12_Event_Trigger_Template"/>
  </rdf:Property>
  <rdf:Property rdf:about="https://takin.solutions/ontologies/CRMcpr/CP15i_is_sub-event_stipulated_by">
    <rdfs:domain rdf:resource="https://takin.solutions/ontologies/CRMcpr/CC12_Event_Trigger_Template"/>
    <rdfs:comment xml:lang="en">This property is the inverse of the forward property described in the scope note that follows. This property enables the documentation of planned sub-events stipulated as part of an overall projected event. It is used to link an instance of Event Trigger Template to another instance of this class which would be an element of its own execution. The intention of this property is to enable the modelling of the projection of a complex event with sub-elements.</rdfs:comment>
    <rdfs:label xml:lang="en">is sub-event stipulated by</rdfs:label>
    <skos:notation rdf:datatype="http://www.w3.org/2001/XMLSchema#string">CP15i</skos:notation>
    <rdfs:range rdf:resource="https://takin.solutions/ontologies/CRMcpr/CC12_Event_Trigger_Template"/>
  </rdf:Property>
  <rdf:Property rdf:about="https://takin.solutions/ontologies/CRMcpr/CP16i_is_material_stipulated_by">
    <rdfs:domain rdf:resource="http://www.cidoc-crm.org/cidoc-crm/E57_Material"/>
    <rdfs:comment xml:lang="en">This property is the inverse of the forward property described in the scope note that follows. This property describes the material of which the projected object is expected to be comprised.</rdfs:comment>
    <rdfs:label xml:lang="en">is material stipulated by</rdfs:label>
    <skos:notation rdf:datatype="http://www.w3.org/2001/XMLSchema#string">CP16i</skos:notation>
    <rdfs:range rdf:resource="https://takin.solutions/ontologies/CRMcpr/CC11_Object_Trigger_Template"/>
  </rdf:Property>
  <rdf:Property rdf:about="https://takin.solutions/ontologies/CRMcpr/CP17i_is_site_stipulated_by">
    <rdfs:domain rdf:resource="http://www.cidoc-crm.org/cidoc-crm/E27_Site"/>
    <rdfs:comment xml:lang="en">This property is the inverse of the forward property described in the scope note that follows. This property describes a particular real world site at which the projected object is expected to be installed or placed.</rdfs:comment>
    <rdfs:label xml:lang="en">is site stipulated by</rdfs:label>
    <skos:notation rdf:datatype="http://www.w3.org/2001/XMLSchema#string">CP17i</skos:notation>
    <rdfs:range rdf:resource="https://takin.solutions/ontologies/CRMcpr/CC11_Object_Trigger_Template"/>
  </rdf:Property>
  <rdf:Property rdf:about="https://takin.solutions/ontologies/CRMcpr/CP18i_is_dimension_stipulated_by">
    <rdfs:domain rdf:resource="http://www.cidoc-crm.org/cidoc-crm/E54_Dimension"/>
    <rdfs:comment xml:lang="en">This property is the inverse of the forward property described in the scope note that follows. This property describes the expected dimensions of the projected object.</rdfs:comment>
    <rdfs:label xml:lang="en">is dimension stipulated by</rdfs:label>
    <skos:notation rdf:datatype="http://www.w3.org/2001/XMLSchema#string">CP18i</skos:notation>
    <rdfs:range rdf:resource="https://takin.solutions/ontologies/CRMcpr/CC11_Object_Trigger_Template"/>
  </rdf:Property>
  <rdf:Property rdf:about="https://takin.solutions/ontologies/CRMcpr/CP19i_is_function_stipulated_by">
    <rdfs:domain rdf:resource="http://www.cidoc-crm.org/cidoc-crm/E55_Type"/>
    <rdfs:comment xml:lang="en">This property is the inverse of the forward property described in the scope note that follows. This property describes the expected function of the projected object.</rdfs:comment>
    <rdfs:label xml:lang="en">is function stipulated by</rdfs:label>
    <skos:notation rdf:datatype="http://www.w3.org/2001/XMLSchema#string">CP19i</skos:notation>
    <rdfs:range rdf:resource="https://takin.solutions/ontologies/CRMcpr/CC11_Object_Trigger_Template"/>
  </rdf:Property>
  <rdf:Property rdf:about="https://takin.solutions/ontologies/CRMcpr/CP20i_is_reference_stipulated_by">
    <rdfs:domain rdf:resource="http://www.cidoc-crm.org/cidoc-crm/E73_Information_Object"/>
    <rdfs:comment xml:lang="en">This property is the inverse of the forward property described in the scope note that follows. This property associates an instance of Object Trigger Template with an Information Object which is to be used as a reference in the making of the projected object. The end result should show similarity to the referenced object</rdfs:comment>
    <rdfs:label xml:lang="en">is reference stipulated by</rdfs:label>
    <skos:notation rdf:datatype="http://www.w3.org/2001/XMLSchema#string">CP20i</skos:notation>
    <rdfs:range rdf:resource="https://takin.solutions/ontologies/CRMcpr/CC11_Object_Trigger_Template"/>
  </rdf:Property>
  <rdf:Property rdf:about="https://takin.solutions/ontologies/CRMcpr/CP21i_is_part_stipulated_by">
    <rdfs:domain rdf:resource="https://takin.solutions/ontologies/CRMcpr/CC11_Object_Trigger_Template"/>
    <rdfs:comment xml:lang="en">This property is the inverse of the forward property described in the scope note that follows. This property enables the documentation of expected parts of a planned object and the particular features of those parts.</rdfs:comment>
    <rdfs:label xml:lang="en">is part stipulated by</rdfs:label>
    <skos:notation rdf:datatype="http://www.w3.org/2001/XMLSchema#string">CP21i</skos:notation>
    <rdfs:range rdf:resource="https://takin.solutions/ontologies/CRMcpr/CC11_Object_Trigger_Template"/>
  </rdf:Property>
  <rdf:Property rdf:about="https://takin.solutions/ontologies/CRMcpr/CP22i_was_assessed_by">
    <rdfs:domain rdf:resource="http://www.cidoc-crm.org/cidoc-crm/E73_Information_Object"/>
    <rdfs:comment xml:lang="en">This property is the inverse of the forward property described in the scope note that follows. This property indicates that an assessment activity was carried out on an instance of information object.</rdfs:comment>
    <rdfs:label xml:lang="en">was assessed by</rdfs:label>
    <skos:notation rdf:datatype="http://www.w3.org/2001/XMLSchema#string">CP22i</skos:notation>
    <rdfs:range rdf:resource="https://takin.solutions/ontologies/CRMcpr/CC19_Assessment"/>
  </rdf:Property>
  <rdf:Property rdf:about="https://takin.solutions/ontologies/CRMcpr/CP24i_was_revision_produced_by">
    <rdfs:domain rdf:resource="http://www.cidoc-crm.org/cidoc-crm/E73_Information_Object"/>
    <rdfs:comment xml:lang="en">This property is the inverse of the forward property described in the scope note that follows. This property indicates that a new information object was created out of an assessment activity. The generated instance of information object will incorporate the assessed information object but may have added, removed, or modified its content as part of the assessment activity.</rdfs:comment>
    <rdfs:label xml:lang="en">was revision produced by</rdfs:label>
    <skos:notation rdf:datatype="http://www.w3.org/2001/XMLSchema#string">CP24i</skos:notation>
    <rdfs:range rdf:resource="https://takin.solutions/ontologies/CRMcpr/CC19_Assessment"/>
  </rdf:Property>
  <rdf:Property rdf:about="https://takin.solutions/ontologies/CRMcpr/CP25i_is_object_of_concern_of">
    <rdfs:domain rdf:resource="http://www.cidoc-crm.org/cidoc-crm/E18_Physical_Thing"/>
    <rdfs:comment xml:lang="en">This property is the inverse of the forward property described in the scope note that follows. This property describes instances of things that are the main object concerned in the realization of the projected new configuration of an extant object. The execution of the object template may result in modification or transformation of the object indicated by this property.</rdfs:comment>
    <rdfs:label xml:lang="en">is object of concern of</rdfs:label>
    <skos:notation rdf:datatype="http://www.w3.org/2001/XMLSchema#string">CP25i</skos:notation>
    <rdfs:range rdf:resource="https://takin.solutions/ontologies/CRMcpr/CC11_Object_Trigger_Template"/>
  </rdf:Property>
    
</rdf:RDF>
